5-15 changes (towards updating Mathlib)

FormalizationOfComputability/ComputableSeq.lean
@@ -10,29 +10,44 @@ namespace Computability
 
 /- Given that S is infinitely often some, produce the index of the next some element, starting at s -/
 def seekSomeIndex {α} (S : Stream' (Option α)) [DecidablePred (fun t => ∃ n, S t = some n)]
-    (h : ∀ N, ∃ t ≥ N, ∃ n, S t = some n) (s : ℕ) : ℕ :=
-  Nat.find (h s)
+  (h : ∀ N, ∃ t ≥ N, ∃ n, S t = some n) (s : ℕ) : ℕ :=
+    Nat.find (h s)
+
+/- Finding the next some element of an infinite Stream' is computable. -/
+lemma computable_seekSomeIndex {α} [Primcodable α] (S : Stream' (Option α))
+  [DecidablePred (fun t ↦ ∃ n, S t = some n)] (h : ∀ N, ∃ t ≥ N, ∃ n, S t = some n)
+  (hP : ComputablePred fun p : ℕ × ℕ => p.1 ≤ p.2 ∧ ∃ n, S p.2 = some n) :
+    Computable fun s ↦ seekSomeIndex S h s := by
+  let q : ℕ → ℕ → Bool := fun s t ↦ decide (s ≤ t ∧ ∃ n, S t = some n)
+  obtain ⟨x, hq₀⟩ := hP
+  refine Partrec.of_eq_tot (Partrec.rfind (hq₀.to₂).partrec₂) ?_
+  intro s
+  rw [Nat.mem_rfind]
+  dsimp [q, seekSomeIndex]
+  constructor
+  · simp [Nat.find_spec (h s)]
+  · intro m hm
+    simp [Nat.find_min (h s) hm]
 
 /- Given that S is infinitely often some, produce the next some element, starting at s -/
-def seekSome {α} (S : Stream' (Option α))
-    [DecidablePred (fun t => ∃ n, S t = some n)]
-    (h : ∀ N, ∃ t ≥ N, ∃ n, S t = some n) (s : ℕ) : α :=
-  (S (Nat.find (h s))).get
-    (by exact Option.isSome_iff_exists.mpr ((Nat.find_spec (h s)).2))
+def seekSome {α} (S : Stream' (Option α)) [DecidablePred (fun t => ∃ n, S t = some n)]
+  (h : ∀ N, ∃ t ≥ N, ∃ n, S t = some n) (s : ℕ) : α :=
+    (S (Nat.find (h s))).get
+  (by exact Option.isSome_iff_exists.mpr ((Nat.find_spec (h s)).2))
 
 lemma seekSome_spec {α} (S : Stream' (Option α)) [DecidablePred (fun t => ∃ n, S t = some n)]
-    (h : ∀ N, ∃ t ≥ N, ∃ n, S t = some n) (s : ℕ) :
+  (h : ∀ N, ∃ t ≥ N, ∃ n, S t = some n) (s : ℕ) :
     S (seekSomeIndex S h s) = some (seekSome S h s) := by
   simp only [seekSomeIndex, ge_iff_le, seekSome, Option.some_get]
 
 /- The index found by seekSomeIndex is at or after the input index. -/
 lemma seekSomeIndex_gt {α} (S : Stream' (Option α)) [DecidablePred (fun t => ∃ n, S t = some n)]
-    (h : ∀ N, ∃ t ≥ N, ∃ n, S t = some n) (s : ℕ) :
+  (h : ∀ N, ∃ t ≥ N, ∃ n, S t = some n) (s : ℕ) :
     seekSomeIndex S h s ≥ s := by
   exact (Nat.find_spec (h s)).1
 
 lemma seekSomeIndex_eq_self {α} (S : Stream' (Option α)) [DecidablePred (fun t => ∃ n, S t = some n)]
-    (h : ∀ N, ∃ t ≥ N, ∃ n, S t = some n) {s : ℕ} {a : α} (hs : S s = some a) :
+  (h : ∀ N, ∃ t ≥ N, ∃ n, S t = some n) {s : ℕ} {a : α} (hs : S s = some a) :
     seekSomeIndex S h s = s := by
   apply le_antisymm
   · exact Nat.find_min' (h s) ⟨le_rfl, ⟨a, hs⟩⟩
@@ -40,36 +55,66 @@ lemma seekSomeIndex_eq_self {α} (S : Stream' (Option α)) [DecidablePred (fun t
 
 -- The index found by seekSomeIndex points to a some value.
 lemma seekSomeIndex_isSome {α} (S : Stream' (Option α)) [DecidablePred (fun t => ∃ n, S t = some n)]
-    (h : ∀ N, ∃ t ≥ N, ∃ n, S t = some n) (s : ℕ) :
+  (h : ∀ N, ∃ t ≥ N, ∃ n, S t = some n) (s : ℕ) :
     ∃ n, S (seekSomeIndex S h s) = some n := by
   exact (Nat.find_spec (h s)).2
 
 /- The indices of the some entries of S. -/
-def dropNoneIndex {α} (S : Stream' (Option α))
-    [DecidablePred (fun t => ∃ n, S t = some n)]
-    (h : ∀ N, ∃ t ≥ N, ∃ n, S t = some n) : ℕ → ℕ
-  | 0 => seekSomeIndex S h 0
-  | s + 1 => seekSomeIndex S h (dropNoneIndex S h s+1)
+def dropNoneIndex {α} (S : Stream' (Option α)) [DecidablePred (fun t => ∃ n, S t = some n)]
+  (h : ∀ N, ∃ t ≥ N, ∃ n, S t = some n) : ℕ → ℕ
+    | 0 => seekSomeIndex S h 0
+    | s + 1 => seekSomeIndex S h (dropNoneIndex S h s+1)
+
+lemma computable_dropNoneIndex {α} [Primcodable α] (S : Stream' (Option α))
+  [DecidablePred (fun t ↦ ∃ n, S t = some n)] (h : ∀ N, ∃ t ≥ N, ∃ n, S t = some n)
+  (hP : ComputablePred fun p : ℕ × ℕ => p.1 ≤ p.2 ∧ ∃ n, S p.2 = some n) :
+    Computable fun s ↦ dropNoneIndex S h s := by
+  let seek := seekSomeIndex S h
+  have hseek := computable_seekSomeIndex S h hP
+  have hrec : Computable fun s : ℕ => Nat.rec (motive := fun _ => ℕ)
+      (seek 0) (fun _ IH => seek (IH + 1)) s := by
+    let step : ℕ → ℕ × ℕ → ℕ := fun _ p => seek (p.2 + 1)
+    have hstep : Computable₂ step := by
+      apply Computable₂.mk
+      dsimp [step]
+      exact hseek.comp <| Computable.succ.comp <| Computable.snd.comp Computable.snd
+    simpa [step] using
+    (Computable.nat_rec (α := ℕ) (σ := ℕ) (f := fun s : ℕ => s) (g := fun _ : ℕ => seek 0)
+      (h := step) Computable.id (Computable.const (seek 0)) hstep)
+  refine hrec.of_eq ?_
+  intro s
+  induction s with
+  | zero =>
+      rfl
+  | succ s ih =>
+      simp [dropNoneIndex, seek, ih]
 
 -- The stream obtained from S by deleting all the none entries.
 def dropNone {α} (S : Stream' (Option α)) [DecidablePred (fun t => ∃ n, S t = some n)]
-    (h : ∀ N, ∃ t ≥ N, ∃ n, S t = some n) : Stream' α :=
-  fun s =>
-    Option.get (S (dropNoneIndex S h s)) <| by
-    apply Option.isSome_iff_exists.mpr
-    unfold dropNoneIndex
-    cases s with | zero | succ s
-    <;> simp [seekSome_spec S h ?_]
+  (h : ∀ N, ∃ t ≥ N, ∃ n, S t = some n) : Stream' α :=
+    fun s => Option.get (S (dropNoneIndex S h s)) <| by
+  apply Option.isSome_iff_exists.mpr
+  unfold dropNoneIndex
+  cases s with | zero | succ s
+  <;> simp [seekSome_spec S h ?_]
 
 /- The value of dropNone at index s agrees with the original stream at index dropNoneIndex S h s. -/
 lemma dropNone_spec {α} (S : Stream' (Option α)) [DecidablePred (fun t => ∃ n, S t = some n)]
-    (h : ∀ N, ∃ t ≥ N, ∃ n, S t = some n) (s : ℕ) :
+  (h : ∀ N, ∃ t ≥ N, ∃ n, S t = some n) (s : ℕ) :
     S (dropNoneIndex S h s) = some (dropNone S h s) := by
   simp only [dropNone, Option.some_get]
 
+lemma computable_dropNone {α} [Primcodable α] (S : Stream' (Option α))
+  [DecidablePred (fun t ↦ ∃ n, S t = some n)] (h : ∀ N, ∃ t ≥ N, ∃ n, S t = some n)
+  (hS : Computable S) (hP : ComputablePred fun p : ℕ × ℕ => p.1 ≤ p.2 ∧ ∃ n, S p.2 = some n) :
+    Computable fun s ↦ dropNone S h s := by
+  refine Partrec.of_eq_tot (Computable.ofOption (hS.comp (computable_dropNoneIndex S h hP))) ?_
+  intro s
+  simp only [dropNone_spec, Part.coe_some, Part.mem_some_iff]
+
 /- The indices selected by dropNoneIndex strictly increase. -/
 lemma dropNoneIndex_gt {α} (S : Stream' (Option α)) [DecidablePred (fun t => ∃ n, S t = some n)]
-    (h : ∀ N, ∃ t ≥ N, ∃ n, S t = some n) (s : ℕ) :
+  (h : ∀ N, ∃ t ≥ N, ∃ n, S t = some n) (s : ℕ) :
     dropNoneIndex S h (s + 1) > dropNoneIndex S h s := by
   change seekSomeIndex S h (dropNoneIndex S h s + 1) > dropNoneIndex S h s
   exact seekSomeIndex_gt S h (dropNoneIndex S h s + 1)
@@ -80,14 +125,13 @@ lemma dropNoneIndex_gt {α} (S : Stream' (Option α)) [DecidablePred (fun t => �
   exact seekSomeIndex_gt S h 0 -/
 
 -- The number of some entries occurring strictly before a given index in the stream.
-def countSomeBefore {α} (S : Stream' (Option α))
-  [DecidablePred (fun t => ∃ n, S t = some n)] : ℕ → ℕ
+def countSomeBefore {α} (S : Stream' (Option α)) [DecidablePred (fun t => ∃ n, S t = some n)] : ℕ → ℕ
   | 0 => 0
   | s + 1 => countSomeBefore S s + if ∃ n, S s = some n then 1 else 0
 
 /- The next some after s in S occurs at the (countSomeBefore S s)th element of dropNone S h. -/
 lemma dropNone_countSome {α} (S : Stream' (Option α)) [DecidablePred (fun t => ∃ n, S t = some n)]
-    (h : ∀ N, ∃ t ≥ N, ∃ n, S t = some n) (s : ℕ) :
+  (h : ∀ N, ∃ t ≥ N, ∃ n, S t = some n) (s : ℕ) :
     seekSomeIndex S h s = dropNoneIndex S h (countSomeBefore S s) := by
   rw [eq_comm]
   induction s with
@@ -111,14 +155,14 @@ lemma dropNone_countSome {α} (S : Stream' (Option α)) [DecidablePred (fun t =>
           simp
 
 lemma dropNone_of_some {α} (S : Stream' (Option α)) [DecidablePred (fun t => ∃ n, S t = some n)]
-    (h : ∀ N, ∃ t ≥ N, ∃ n, S t = some n) {s : ℕ} {a : α} (hs : S s = some a) :
+  (h : ∀ N, ∃ t ≥ N, ∃ n, S t = some n) {s : ℕ} {a : α} (hs : S s = some a) :
     dropNone S h (countSomeBefore S s) = S s := by
   rw [← dropNone_spec S h (countSomeBefore S s), ← dropNone_countSome S h s,
     seekSomeIndex_eq_self S h hs]
 
 /- dropNone S enumerates the same elements as S -/
 lemma dropNoneIff {α} (S : Stream' (Option α)) [DecidablePred (fun t => ∃ n, S t = some n)]
-    (h : ∀ N, ∃ t ≥ N, ∃ n, S t = some n) (a : α) :
+  (h : ∀ N, ∃ t ≥ N, ∃ n, S t = some n) (a : α) :
     (∃ s, S s = some a) ↔ (∃ t, dropNone S h t = a) := by
   constructor
   · intro ⟨s, hs⟩
@@ -128,7 +172,6 @@ lemma dropNoneIff {α} (S : Stream' (Option α)) [DecidablePred (fun t => ∃ n,
   · intro ⟨t, ht⟩
     refine ⟨dropNoneIndex S h t, ?_⟩
     rw [dropNone_spec S h t, ht]
-
 
 lemma Wenum_aux (e : ℕ) (h : (W e).Infinite) : ∀ N, ∃ t ≥ N, ∃ n, (Wenum e) t = some n := by
   exact ((We_infinite_TFAE e).out 0 5).mp h
@@ -147,6 +190,20 @@ lemma Wenum'_mem (e n : ℕ) (h : (W e).Infinite) :
   unfold Wenum'
   simp_all only [dropNoneIff (Wenum e) (Wenum_aux e h)]
 
+lemma computable_Wenum' (e : ℕ) (h : (W e).Infinite) :
+    Computable fun x ↦ Wenum' e h x := by
+  change Computable fun x ↦ dropNone (Wenum e) (Wenum_aux e h) x
+  apply computable_dropNone
+  · sorry
+  · have h1 := Wenum_dec e
+
+
+instance Wenum'_dec (e : ℕ) (h : (W e).Infinite) : ComputablePred fun (n, s) ↦ Wenum' e h s = n := by
+  simp
+  unfold ComputablePred
+  have hP := computable_Wenum' e h
+
+
 
 def Pi01 (X : Set ℕ): Prop := Sigma01 Xᶜ
 
@@ -164,34 +221,13 @@ theorem delta01_iff_sigma01_and_pi01 (X : Set ℕ) : Delta01 X ↔ Sigma01 X ∧
     rw [Computable.set_iff_ComputablePred, ComputablePred.computable_iff_re_compl_re']
     simp_all [Partrec.set_iff_REPred]
 
-/- If W e is infinite, eventually every emitted element is greater than x.-/
-lemma inf_inc_exists_pass (e x : ℕ) (h : (W e).Infinite)
-    (hinc : ∀ m n, m < n → Wenum' e h m < Wenum' e h n) :
-    ∃ N, x < Wenum' e h N := by
-  obtain ⟨y, hyW, hxy⟩ := Set.Infinite.exists_gt h x
-  have ⟨N, hN⟩ : ∃ N, Wenum' e h N = y := by
-    rw [← Wenum'_mem]
-    grind [(We_mem_TFAE e y).out 0 3]
-  refine ⟨N + 1, ?_⟩
-  simp only [lt_trans hxy, ← hN, hinc, lt_add_iff_pos_right, zero_lt_one]
-
-/- Recursively find the first index s for which Wenum' e s > x -/
-def firstPassIndex (e x : ℕ) (h : (W e).Infinite)
-    (hinc : ∀ m n, m < n → Wenum' e h m < Wenum' e h n) : ℕ :=
-  Nat.find (inf_inc_exists_pass e x h hinc)
-
-/- The firstPassIndex really does pass x. -/
-lemma firstPassIndex_spec (e x : ℕ) (h : (W e).Infinite)
-    (hinc : ∀ m n, m < n → Wenum' e h m < Wenum' e h n) :
-    x < Wenum' e h (firstPassIndex e x h hinc) :=
-  Nat.find_spec (inf_inc_exists_pass e x h hinc)
-
-/- firstPassIndex is minimal among indices whose emitted value is greater than x. -/
-lemma firstPassIndex_min (e x : ℕ) (h : (W e).Infinite)
-    (hinc : ∀ m n, m < n → Wenum' e h m < Wenum' e h n)
-    {s : ℕ} (hs : x < Wenum' e h s) :
-    firstPassIndex e x h hinc ≤ s :=
-  Nat.find_min' (inf_inc_exists_pass e x h hinc) hs
+/- If W e is infinite and increasing, every emitted element is at least its index -/
+lemma inc_ge_index (e : ℕ) (h : (W e).Infinite) (hinc : ∀ m n, m < n → Wenum' e h m < Wenum' e h n) :
+    ∀ s, s ≤ Wenum' e h s := by
+  intro s
+  induction s with | zero | succ s ih
+  · exact Nat.zero_le _
+  · exact Nat.succ_le_of_lt (lt_of_le_of_lt ih (hinc s (s + 1) (Nat.lt_succ_self s)))
 
 lemma inf_inc_sigma01_is_delta01 (e : ℕ) (h : (W e).Infinite)
   (hinc : ∀ m n, m < n → Wenum' e h m < Wenum' e h n) :
@@ -199,26 +235,20 @@ lemma inf_inc_sigma01_is_delta01 (e : ℕ) (h : (W e).Infinite)
   have hmem (x : ℕ) : x ∈ W e ↔ ∃ n, Wenum' e h n = x := by
     rw [← Wenum'_mem]
     grind [(We_mem_TFAE e x).out 0 3]
-  let N (x : ℕ) := firstPassIndex e x h hinc
-  have hx (x : ℕ) : x ∈ W e ↔ (∃ s < N x, Wenum' e h s = x) := by
+  have hx (x : ℕ) : x ∈ W e ↔ (∃ s < x+1, Wenum' e h s = x) := by
     constructor
     <;> intro h1
     · obtain ⟨s, h1⟩ := (hmem x).mp h1
       refine ⟨s, ⟨?_, h1⟩⟩
-      unfold N
-      have hpass := firstPassIndex_spec e x h hinc
-      by_contra hsN
-      apply Nat.le_of_not_gt at hsN
-      rcases Nat.lt_or_eq_of_le hsN
-      <;> grind
+      have hs := inc_ge_index e h hinc s
+      rw [h1] at hs
+      exact Nat.lt_succ_of_le hs
     · obtain ⟨s, ⟨_, h2⟩⟩ := h1
       apply (hmem x).mpr
       use s
   refine (Computable.set_iff_ComputablePred (W e)).mpr ?_
-  -- now membership in W e is equivalent to a bounded search, so it is computable!
-  sorry
-
-
+  simp_rw [hx, ← Finset.mem_range, ← Finset.mem_toList]
+  have hR : ComputablePred fun (n, s) ↦ Wenum' e h s = n := Wenum'_dec e h
 
 
 
